\begin{answer}
\begin{align*}
d^* &= \arg\max_d \ell(\theta) + d^T\nabla_{\theta'}\ell(\theta')|_{\theta'=\theta} \quad \text{subject to} \quad 
\frac{1}{2}d^T \mathcal{I}(\theta) d = c
\end{align*}
\[\mathcal{L}(d, \lambda) = \log p(y; \theta) + d^T\nabla_{\theta'}\log p(y; \theta')|_{\theta'=\theta} - \lambda  [\frac{1}{2}d^T \mathcal{I}(\theta) d - c]\]
We calculate the derivatives of $\mathcal{L}(d, \lambda)$ with respect to $d, \lambda$
\begin{align*}
    \frac{\partial \mathcal{L}(d, \lambda)}{\partial d} &= \nabla_{\theta'}\log p(y; \theta')|_{\theta'=\theta} - \lambda \mathcal{I}(\theta) d\\
    \frac{\partial \mathcal{L}(d, \lambda)}{\partial \lambda} &= -\frac{1}{2}d^T \mathcal{I}(\theta) d + c\\
\end{align*}
By setting the first partial derivative to zero, we can get:
$$d = \frac{1}{\lambda} \mathcal{I}(\theta)^{-1} \nabla_{\theta'}\log p(y; \theta')|_{\theta'=\theta}$$
We plugin the above expression for $d$ into the second partial derivative and set it to zero.
\begin{align*}
    &\frac{1}{2}(\frac{1}{\lambda} \mathcal{I}(\theta)^{-1} \nabla_{\theta'}\log p(y; \theta')|_{\theta'=\theta})^T \mathcal{I}(\theta) (\frac{1}{\lambda} \mathcal{I}(\theta)^{-1} \nabla_{\theta'}\log p(y; \theta')|_{\theta'=\theta}) = c\\
    &\lambda = \sqrt{\frac{1}{2c} (\nabla_{\theta'}\log p(y; \theta')|_{\theta'=\theta})^T \mathcal{I}(\theta)^{-1} (\nabla_{\theta'}\log p(y; \theta')|_{\theta'=\theta}})
\end{align*}
Plug that expression for $\lambda$ back into unscaled $d$:
$$d^* = \sqrt{\frac{2c}{(\nabla_{\theta'}\log p(y; \theta')|_{\theta'=\theta})^T \mathcal{I}(\theta)^{-1} (\nabla_{\theta'}\log p(y; \theta')|_{\theta'=\theta})}} \mathcal{I}(\theta)^{-1} \nabla_{\theta'}\log p(y; \theta')|_{\theta'=\theta}$$
\end{answer}
