\begin{answer}
\begin{align*}
    l(\theta) = \log P(y;\eta) = -\log b(y)-\eta^T T(y)+a(\eta)\\
    =-\log b(y) - \theta^T x y + a(\theta^T x)
\end{align*}
the first and second derivatives of $l(\theta)$ are:
\begin{align*}
    \frac{\partial l(\theta)}{\partial \theta_j} &= -y x_i + a'(\theta^T x)x_i\\
    \frac{\partial^2 l(\theta)}{\partial \theta_i \partial \theta_j} &= a''(\theta^T x)x_i x_j
\end{align*}
So, the Hessian matrix is $H = \frac{\partial^2 l(\theta)}{\partial \theta^2} = a''(\theta^T x) x x^T$
\begin{align*}
    \forall z \in \mathbb{R}^n, z^T H z &= a''(\theta^T x) z^T x x^T z\\
    &= a''(\theta^T x) (x^T z)^2 \geq 0
\end{align*}
\end{answer}
