\begin{answer}
\begin{align*}
    P(y=1|x;\phi, \mu_0, \mu_1, \Sigma) &= \frac{P(y=1)P(x|y=1)}{P(y=0)P(x|y=0)+P(y=1)P(x|y=1)}\\
    &= \frac{\phi exp(-\frac{1}{2}(x-\mu_1)^T\Sigma^{-1}(x-\mu_1))}{\phi exp(-\frac{1}{2}(x-\mu_1)^T\Sigma^{-1}(x-\mu_1)) + (1 - \phi) exp(-\frac{1}{2}(x-\mu_0)^T\Sigma^{-1}(x-\mu_0))}\\
    &= \frac{1}{1 + \frac{1-\phi}{\phi}exp(-\frac{1}{2}(x-\mu_0)^T\Sigma^{-1}(x-\mu_0)+\frac{1}{2}(x-\mu_1)^T\Sigma^{-1}(x-\mu_1))}\\
    &=\frac{1}{1+exp(log\frac{1-\phi}{\phi} + \mu_0^T\Sigma^{-1}x - \mu_1^T\Sigma^{-1}x + \frac{1}{2}(\mu_1^T\Sigma^{-1}\mu_1 - \mu_0^T\Sigma^{-1}\mu_0)}
\end{align*}
So, the following formula are $\theta$ and $\theta_0$:
\begin{align*}
    \theta &= \Sigma^{-1}(\mu_1-\mu_0)\\
    \theta_0 &= log\frac{\phi}{1 - \phi} + \frac{1}{2}(\mu_0^T\Sigma^{-1}\mu_0 - \mu_1^T\Sigma^{-1}\mu_1)
\end{align*}
\end{answer}
